src/proofs/no_slashable_attestations/supporting_lemmas/dv_next_preserves_ind_inv/invs_fnc_2.dfy
@@ -2001,7 +2001,7 @@ module Fnc_Invs_2
                     set signer, att_share | 
                         && att_share in att_shares
                         && signer in dv.all_nodes
-                        && verify_bls_siganture(signing_root, att_share.signature, signer)
+                        && verify_bls_signature(signing_root, att_share.signature, signer)
                     ::
                         signer;
             && exists hn :: hn in signers && is_honest_node(dv, hn)
@@ -2012,7 +2012,7 @@ module Fnc_Invs_2
                     set signer, att_share | 
                         && att_share in att_shares
                         && signer in all_nodes
-                        && verify_bls_siganture(signing_root, att_share.signature, signer)
+                        && verify_bls_signature(signing_root, att_share.signature, signer)
                     ::
                         signer;
 
@@ -2245,4 +2245,436 @@ module Fnc_Invs_2
                 process'.dv_pubkey
                 )
     { }  
+
+    lemma lem_inv_outputs_attestations_submited_is_created_with_shares_from_quorum_f_start_next_duty(
+        process: DVCState, 
+        attestation_duty: AttestationDuty, 
+        process': DVCState
+    )
+    requires f_start_next_duty.requires(process, attestation_duty)
+    requires process' == f_start_next_duty(process, attestation_duty).state    
+    ensures inv_outputs_attestations_submited_is_created_with_shares_from_quorum(                
+                f_start_next_duty(process, attestation_duty).outputs,
+                process'
+            )
+    { }  
+
+    lemma lem_inv_outputs_attestations_submited_is_created_with_shares_from_quorum_f_check_for_next_duty(
+        process: DVCState,
+        attestation_duty: AttestationDuty,
+        process': DVCState
+    )
+    requires f_check_for_next_duty.requires(process, attestation_duty)
+    requires process' == f_check_for_next_duty(process, attestation_duty).state
+    ensures inv_outputs_attestations_submited_is_created_with_shares_from_quorum(
+                f_check_for_next_duty(process, attestation_duty).outputs,
+                process'
+            )
+    { }
+
+    lemma lem_inv_outputs_attestations_submited_is_created_with_shares_from_quorum_f_serve_attestation_duty(
+        process: DVCState,
+        attestation_duty: AttestationDuty,
+        process': DVCState
+    )  
+    requires f_serve_attestation_duty.requires(process, attestation_duty)
+    requires process' == f_serve_attestation_duty(process, attestation_duty).state
+    ensures inv_outputs_attestations_submited_is_created_with_shares_from_quorum(
+                f_serve_attestation_duty(process, attestation_duty).outputs,
+                process'
+            )
+    {
+        var process_rcvd_duty := 
+                process.(all_rcvd_duties := process.all_rcvd_duties + {attestation_duty});
+        var process_after_stopping_active_consensus_instance := f_terminate_current_attestation_duty(process_rcvd_duty);
+        lem_inv_outputs_attestations_submited_is_created_with_shares_from_quorum_f_check_for_next_duty(
+            process_after_stopping_active_consensus_instance,
+            attestation_duty,
+            process'
+        );   
+    } 
+
+    lemma lem_inv_outputs_attestations_submited_is_created_with_shares_from_quorum_f_listen_for_new_imported_blocks(
+        process: DVCState,
+        block: BeaconBlock,
+        process': DVCState
+    )
+    requires f_listen_for_new_imported_blocks.requires(process, block)
+    requires process' == f_listen_for_new_imported_blocks(process, block).state
+    ensures inv_outputs_attestations_submited_is_created_with_shares_from_quorum(
+                f_listen_for_new_imported_blocks(process, block).outputs,
+                process'
+            )
+    { }  
+
+    lemma lem_inv_outputs_attestations_submited_is_created_with_shares_from_quorum_f_listen_for_attestation_shares(
+        process: DVCState,
+        attestation_share: AttestationShare,
+        process': DVCState
+    )
+    requires f_listen_for_attestation_shares.requires(process, attestation_share)
+    requires process' == f_listen_for_attestation_shares(process, attestation_share).state
+    requires construct_signed_attestation_signature_assumptions_helper(
+                process.construct_signed_attestation_signature,
+                process.dv_pubkey,
+                process.peers
+             )
+    ensures inv_outputs_attestations_submited_is_created_with_shares_from_quorum(
+                f_listen_for_attestation_shares(process, attestation_share).outputs,
+                process'
+                )
+    { 
+        var activate_att_consensus_intances := process.attestation_consensus_engine_state.active_attestation_consensus_instances.Keys;
+
+        if  || (activate_att_consensus_intances == {} && !process.latest_attestation_duty.isPresent())
+            || (activate_att_consensus_intances != {} && minInSet(activate_att_consensus_intances) <= attestation_share.data.slot)
+            || (activate_att_consensus_intances == {} && !process.current_attestation_duty.isPresent() && process.latest_attestation_duty.isPresent() && process.latest_attestation_duty.safe_get().slot < attestation_share.data.slot) 
+        {
+            var k := (attestation_share.data, attestation_share.aggregation_bits);
+            var attestation_shares_db_at_slot := getOrDefault(process.rcvd_attestation_shares, attestation_share.data.slot, map[]);
+            
+            var new_attestation_shares_db := 
+                    process.rcvd_attestation_shares[
+                        attestation_share.data.slot := 
+                            attestation_shares_db_at_slot[
+                                        k := 
+                                            getOrDefault(attestation_shares_db_at_slot, k, {}) + 
+                                            {attestation_share}
+                                        ]
+                            ];
+
+            var process_with_new_att_shares_db := 
+                    process.(
+                        rcvd_attestation_shares := new_attestation_shares_db
+                    );
+
+                        
+            if process_with_new_att_shares_db.construct_signed_attestation_signature(process_with_new_att_shares_db.rcvd_attestation_shares[attestation_share.data.slot][k]).isPresent() 
+            {
+                var aggregated_attestation := 
+                    f_construct_aggregated_attestation_for_new_attestation_share(
+                        attestation_share,
+                        k, 
+                        process_with_new_att_shares_db.construct_signed_attestation_signature,
+                        process_with_new_att_shares_db.rcvd_attestation_shares
+                    );
+
+                var new_outputs := getEmptyOuputs().(
+                                            attestations_submitted := {aggregated_attestation} 
+                                        );
+
+                var process_after_submitting_attestations := 
+                    process_with_new_att_shares_db.(
+                        bn := process_with_new_att_shares_db.bn.(
+                            attestations_submitted := process_with_new_att_shares_db.bn.attestations_submitted + [aggregated_attestation]
+                        )
+                    );
+
+                assert  process.construct_signed_attestation_signature
+                        ==
+                        process_after_submitting_attestations.construct_signed_attestation_signature
+                        ;
+
+                assert  && process.dv_pubkey == process_after_submitting_attestations.dv_pubkey
+                        && process.peers == process_after_submitting_attestations.peers;
+
+                var rcvd_attestation_shares := process_with_new_att_shares_db.rcvd_attestation_shares;
+                var construct_signed_attestation_signature := process_with_new_att_shares_db.construct_signed_attestation_signature;
+                
+                assert  &&  attestation_share.data.slot in rcvd_attestation_shares.Keys
+                        &&  k in rcvd_attestation_shares[attestation_share.data.slot]
+                        &&  construct_signed_attestation_signature(rcvd_attestation_shares[attestation_share.data.slot][k]).isPresent()    
+                        &&  do_all_att_shares_have_the_same_data(
+                                rcvd_attestation_shares[attestation_share.data.slot][k], 
+                                aggregated_attestation.data
+                            )
+                        &&  var fork_version := bn_get_fork_version(compute_start_slot_at_epoch(aggregated_attestation.data.target.epoch));
+                        &&  var attestation_signing_root := compute_attestation_signing_root(aggregated_attestation.data, fork_version);      
+                        &&  signer_threshold(
+                                process_with_new_att_shares_db.peers, 
+                                rcvd_attestation_shares[attestation_share.data.slot][k], attestation_signing_root
+                            ) 
+                        &&  aggregated_attestation 
+                            == 
+                            f_construct_aggregated_attestation_for_new_attestation_share(
+                                attestation_share,
+                                k, 
+                                construct_signed_attestation_signature,
+                                rcvd_attestation_shares
+                            )
+                        ;
+            }
+            else 
+            {
+                assert inv_outputs_attestations_submited_is_created_with_shares_from_quorum(
+                            f_listen_for_attestation_shares(process, attestation_share).outputs,
+                            process'
+                            );
+            }
+        }            
+        else 
+        {
+            assert inv_outputs_attestations_submited_is_created_with_shares_from_quorum(
+                        f_listen_for_attestation_shares(process, attestation_share).outputs,
+                        process'
+                        );
+        }
+            
+    }
+
+    lemma lem_inv_outputs_attestations_submited_is_created_with_shares_from_quorum_f_att_consensus_decided(
+        process: DVCState,
+        id: Slot,
+        decided_attestation_data: AttestationData, 
+        process': DVCState
+    )
+    requires f_att_consensus_decided.requires(process, id, decided_attestation_data)
+    requires process' == f_att_consensus_decided(process, id, decided_attestation_data).state 
+    ensures inv_outputs_attestations_submited_is_created_with_shares_from_quorum(
+                f_att_consensus_decided(process, id, decided_attestation_data).outputs,
+                process'
+                )
+    { }  
+
+    lemma lem_inv_db_of_vp_contains_all_att_data_of_sent_att_shares_for_lower_slots_dvc_f_terminate_current_attestation_duty(
+        allMessagesSent: set<AttestationShare>,
+        hn: BLSPubkey,
+        process: DVCState, 
+        process': DVCState
+    )
+    requires f_terminate_current_attestation_duty.requires(process)
+    requires process' == f_terminate_current_attestation_duty(process)
+    requires inv_db_of_vp_contains_all_att_data_of_sent_att_shares_for_lower_slots_dvc(                
+                allMessagesSent,
+                hn,
+                process
+             )
+    ensures inv_db_of_vp_contains_all_att_data_of_sent_att_shares_for_lower_slots_dvc(                
+                allMessagesSent,
+                hn,
+                process'
+            )
+    { }    
+
+    lemma lem_inv_db_of_vp_contains_all_att_data_of_sent_att_shares_for_lower_slots_dvc_f_serve_attestation_duty(
+        allMessagesSent: set<AttestationShare>,
+        hn: BLSPubkey,
+        process: DVCState,
+        attestation_duty: AttestationDuty,
+        process': DVCState
+    )  
+    requires f_serve_attestation_duty.requires(process, attestation_duty)
+    requires process' == f_serve_attestation_duty(process, attestation_duty).state
+     requires inv_db_of_vp_contains_all_att_data_of_sent_att_shares_for_lower_slots_dvc(                
+                allMessagesSent,
+                hn,
+                process
+             )
+    ensures inv_db_of_vp_contains_all_att_data_of_sent_att_shares_for_lower_slots_dvc(                
+                allMessagesSent,
+                hn,
+                process'
+            )
+    {
+        var process_rcvd_duty := 
+                process.(all_rcvd_duties := process.all_rcvd_duties + {attestation_duty});
+        assert  inv_db_of_vp_contains_all_att_data_of_sent_att_shares_for_lower_slots_dvc(                
+                    allMessagesSent,
+                    hn,
+                    process_rcvd_duty
+                );
+        var process_after_stopping_active_consensus_instance := f_terminate_current_attestation_duty(process_rcvd_duty);
+        lem_inv_db_of_vp_contains_all_att_data_of_sent_att_shares_for_lower_slots_dvc_f_terminate_current_attestation_duty(
+            allMessagesSent,
+            hn,
+            process_rcvd_duty,
+            process_after_stopping_active_consensus_instance
+        );
+        lem_inv_db_of_vp_contains_all_att_data_of_sent_att_shares_for_lower_slots_dvc_f_check_for_next_duty(
+            allMessagesSent,
+            hn,
+            process_after_stopping_active_consensus_instance,
+            attestation_duty,
+            process'
+        );   
+    } 
+
+    lemma lem_inv_db_of_vp_contains_all_att_data_of_sent_att_shares_for_lower_slots_dvc_startConsensusInstance_helper(
+        s: ConsensusEngineState,
+        id: Slot,
+        attestation_duty: AttestationDuty,
+        attestation_slashing_db: set<SlashingDBAttestation>,
+        r: ConsensusEngineState
+    )
+    requires id !in s.active_attestation_consensus_instances.Keys
+    requires id == attestation_duty.slot
+    requires r == startConsensusInstance(s, id, attestation_duty, attestation_slashing_db)    
+    ensures &&  var acvc := 
+                AttestationConsensusValidityCheckState(
+                    attestation_duty := attestation_duty,
+                    validityPredicate := (ad: AttestationData) => consensus_is_valid_attestation_data(attestation_slashing_db, ad, attestation_duty)
+                );
+            &&  var vp := acvc.validityPredicate;
+            &&  ( forall slot0, vp0 ::
+                    && var hist_slot0 := getOrDefault(s.att_slashing_db_hist, slot0, map[]);
+                    && var hist_slot_vp0 := getOrDefault(hist_slot0, vp0, {});
+                    && var new_hist_slot0 := getOrDefault(r.att_slashing_db_hist, slot0, map[]);
+                    && var new_hist_slot_vp0 := getOrDefault(new_hist_slot0, vp0, {});
+                    && (( slot0 != id || vp0 != vp )
+                        ==> 
+                        hist_slot_vp0 == new_hist_slot_vp0
+                        )
+                    && ((slot0 == id && vp0 == vp )
+                        ==> 
+                        hist_slot_vp0 + {attestation_slashing_db} == new_hist_slot_vp0
+                        )
+                )
+    { 
+        
+    }  
+
+    lemma lem_inv_db_of_vp_contains_all_att_data_of_sent_att_shares_for_lower_slots_dvc_f_start_next_duty(
+        allMessagesSent: set<AttestationShare>,
+        hn: BLSPubkey,
+        process: DVCState, 
+        attestation_duty: AttestationDuty, 
+        process': DVCState
+    )
+    requires f_start_next_duty.requires(process, attestation_duty)
+    requires process' == f_start_next_duty(process, attestation_duty).state    
+    requires inv_db_of_vp_contains_all_att_data_of_sent_att_shares_for_lower_slots_dvc(                
+                allMessagesSent,
+                hn,
+                process
+             )
+    // ensures inv_db_of_vp_contains_all_att_data_of_sent_att_shares_for_lower_slots_dvc(                
+    //             allMessagesSent,
+    //             hn,
+    //             process'
+    //         )
+    { 
+        var duty_slot := attestation_duty.slot;
+        var attestation_slashing_db := process.attestation_slashing_db;
+        var att_slashing_db_hist: map<Slot, map<AttestationData -> bool, set<set<SlashingDBAttestation>>>> := process.attestation_consensus_engine_state.att_slashing_db_hist;
+        var attestation_slashing_db' := process'.attestation_slashing_db;
+        var att_slashing_db_hist': map<Slot, map<AttestationData -> bool, set<set<SlashingDBAttestation>>>> := process'.attestation_consensus_engine_state.att_slashing_db_hist;
+
+        var acvc := 
+            AttestationConsensusValidityCheckState(
+                attestation_duty := attestation_duty,
+                validityPredicate := (ad: AttestationData) => consensus_is_valid_attestation_data(attestation_slashing_db, ad, attestation_duty)
+            );
+        var new_vp := acvc.validityPredicate;
+        var new_active_attestation_consensus_instances := 
+            process.attestation_consensus_engine_state.active_attestation_consensus_instances[
+                duty_slot := acvc
+            ];       
+        
+        assert  ( forall slot: Slot, vp: AttestationData -> bool ::
+                    && var hist_slot := getOrDefault(att_slashing_db_hist, slot, map[]);
+                    && var hist_slot_vp := getOrDefault(hist_slot, vp, {});
+                    && var new_hist_slot := getOrDefault(att_slashing_db_hist', slot, map[]);
+                    && var new_hist_slot_vp := getOrDefault(new_hist_slot, vp, {});
+                    && (( slot != duty_slot || vp != new_vp )
+                        ==> 
+                        hist_slot_vp == new_hist_slot_vp
+                        )
+                    && ((slot == duty_slot && vp == new_vp )
+                        ==> 
+                        hist_slot_vp + {attestation_slashing_db} == new_hist_slot_vp
+                        )
+                );
+
+        forall slot: Slot, vp: AttestationData -> bool, db: set<SlashingDBAttestation> | 
+            && slot in att_slashing_db_hist'
+            && vp in att_slashing_db_hist'[slot]
+            && db in att_slashing_db_hist'[slot][vp]
+        // ensures inv_db_of_vp_contains_all_att_data_of_sent_att_shares_for_lower_slots_body_dvc(            
+        //             allMessagesSent,
+        //             hn,
+        //             slot,
+        //             vp,
+        //             db
+        //         )
+        {
+            if slot != duty_slot || vp != new_vp
+            {
+                assert inv_db_of_vp_contains_all_att_data_of_sent_att_shares_for_lower_slots_body_dvc(            
+                    allMessagesSent,
+                    hn,
+                    slot,
+                    vp,
+                    db
+                );                
+            }
+            else
+            {
+                var hist_slot := getOrDefault(att_slashing_db_hist, slot, map[]);
+                var hist_slot_vp := getOrDefault(hist_slot, vp, {});
+                var new_hist_slot := getOrDefault(att_slashing_db_hist', slot, map[]);
+                var new_hist_slot_vp := getOrDefault(new_hist_slot, vp, {});
+                
+                assert hist_slot_vp + {attestation_slashing_db} == new_hist_slot_vp;
+
+                if db in hist_slot_vp
+                {
+                    assert inv_db_of_vp_contains_all_att_data_of_sent_att_shares_for_lower_slots_body_dvc(            
+                                allMessagesSent,
+                                hn,
+                                slot,
+                                vp,
+                                db
+                            );    
+                }
+                else
+                {
+
+                }
+            }
+        }
+    }  
+
+    lemma lem_inv_db_of_vp_contains_all_att_data_of_sent_att_shares_for_lower_slots_dvc_f_check_for_next_duty(
+        allMessagesSent: set<AttestationShare>,
+        hn: BLSPubkey,
+        process: DVCState,
+        attestation_duty: AttestationDuty,
+        process': DVCState
+    )
+    requires f_check_for_next_duty.requires(process, attestation_duty)
+    requires process' == f_check_for_next_duty(process, attestation_duty).state
+    requires inv_db_of_vp_contains_all_att_data_of_sent_att_shares_for_lower_slots_dvc(                
+                allMessagesSent,
+                hn,
+                process
+             )
+    ensures inv_db_of_vp_contains_all_att_data_of_sent_att_shares_for_lower_slots_dvc(                
+                allMessagesSent,
+                hn,
+                process'
+            )
+    { }  
+
+
+    lemma lem_inv_db_of_vp_contains_all_att_data_of_sent_att_shares_for_lower_slots_dvc_f_listen_for_new_imported_blocks(
+        allMessagesSent: set<AttestationShare>,
+        hn: BLSPubkey,
+        process: DVCState,
+        block: BeaconBlock,
+        process': DVCState
+    )
+    requires f_listen_for_new_imported_blocks.requires(process, block)
+    requires process' == f_listen_for_new_imported_blocks(process, block).state
+    requires inv_db_of_vp_contains_all_att_data_of_sent_att_shares_for_lower_slots_dvc(                
+                allMessagesSent,
+                hn,
+                process
+             )
+    ensures inv_db_of_vp_contains_all_att_data_of_sent_att_shares_for_lower_slots_dvc(                
+                allMessagesSent,
+                hn,
+                process'
+            )
+    { }  
+
 }
