src/proofs/no_slashable_attestations/supporting_lemmas/ind_inv_implies_safety/core_proofs.dfy
@@ -26,6 +26,7 @@ module Core_Proofs
     import opened DV
     import opened Att_Inv_With_Empty_Initial_Attestation_Slashing_DB
     import opened Invs_DV_Next_3
+    import opened Invs_DV_Next_5
     import opened Helper_Sets_Lemmas
     import opened DVC_Spec_Axioms
 
@@ -53,334 +54,7 @@ module Core_Proofs
 
     }
 
-    lemma lem_no_slashable_submitted_attestations_with_different_slots_i(dv: DVState, a: Attestation, a': Attestation)
-    requires |dv.all_nodes| > 0
-    requires inv_quorum_constraints(dv)   
-    requires inv_unchanged_paras_of_consensus_instances(dv)
-    requires inv_exists_honest_dvc_that_sent_att_share_for_submitted_att(dv)
-    requires inv_data_of_att_share_is_decided_value(dv)
-    requires inv_decided_value_of_consensus_instance_is_decided_by_quorum(dv)    
-    requires && a in dv.all_attestations_created
-             && is_valid_attestation(a, dv.dv_pubkey)
-    requires && a' in dv.all_attestations_created
-             && is_valid_attestation(a', dv.dv_pubkey)
-    requires a.data.slot < a'.data.slot 
-    ensures && var consa := dv.consensus_on_attestation_data[a.data.slot];
-            && var consa' := dv.consensus_on_attestation_data[a'.data.slot];   
-            && exists m: BLSPubkey, h_nodes_a: set<BLSPubkey>, h_nodes_a': set<BLSPubkey> :: 
-                        inv_exists_honest_node_that_contributed_to_decisions_of_consensus_instances(dv, a, a', m, consa, consa', h_nodes_a, h_nodes_a')    
-    {
-        var hna, att_share :|
-                && is_honest_node(dv, hna)
-                && att_share in dv.att_network.allMessagesSent
-                && att_share.data == a.data
-                && var fork_version := bn_get_fork_version(compute_start_slot_at_epoch(att_share.data.target.epoch));
-                && var attestation_signing_root := compute_attestation_signing_root(att_share.data, fork_version);
-                && verify_bls_siganture(attestation_signing_root, att_share.signature, hna);     
-
-        var hna', att_share' :|
-                && is_honest_node(dv, hna)
-                && att_share' in dv.att_network.allMessagesSent
-                && att_share'.data == a'.data
-                && var fork_version := bn_get_fork_version(compute_start_slot_at_epoch(att_share'.data.target.epoch));
-                && var attestation_signing_root := compute_attestation_signing_root(att_share'.data, fork_version);
-                && verify_bls_siganture(attestation_signing_root, att_share'.signature, hna');  
-
-        assert
-                && dv.consensus_on_attestation_data[att_share.data.slot].decided_value.isPresent()
-                && dv.consensus_on_attestation_data[att_share.data.slot].decided_value.safe_get() == att_share.data;       
-
-        assert
-                && dv.consensus_on_attestation_data[att_share'.data.slot].decided_value.isPresent()
-                && dv.consensus_on_attestation_data[att_share'.data.slot].decided_value.safe_get() == att_share'.data;   
-
-        var consa := dv.consensus_on_attestation_data[a.data.slot];
-        var consa' := dv.consensus_on_attestation_data[a'.data.slot];                    
-
-        assert is_a_valid_decided_value(consa); 
-        assert is_a_valid_decided_value(consa');  
-
-        assert consa.decided_value.isPresent();
-
-        var h_nodes_a :| is_a_valid_decided_value_according_to_set_of_nodes(consa, h_nodes_a);
-        var h_nodes_a' :| is_a_valid_decided_value_according_to_set_of_nodes(consa', h_nodes_a');
-
-        assert consa.all_nodes == consa'.all_nodes == dv.all_nodes;
-
-        var nodes := consa.all_nodes;
-        var honest_nodes := consa.honest_nodes_status.Keys;
-        var byz_nodes := nodes - honest_nodes;
-        
-        assert h_nodes_a * byz_nodes == {};
-        assert h_nodes_a' * byz_nodes == {};        
-        assert |h_nodes_a + byz_nodes| >= quorum(|nodes|);
-        assert |h_nodes_a' + byz_nodes| >= quorum(|nodes|);
-        assert |byz_nodes| <= f(|nodes|);
-        assert nodes != {};    
-
-        lemmaQuorumIntersection(nodes, byz_nodes, h_nodes_a + byz_nodes, h_nodes_a' + byz_nodes);
-            
-        var m: BLSPubkey :| m in honest_nodes && m in h_nodes_a && m in h_nodes_a';  
-
-        assert inv_exists_honest_node_that_contributed_to_decisions_of_consensus_instances(dv, a, a', m, consa, consa', h_nodes_a, h_nodes_a');
-        assert ( exists m: BLSPubkey, h_nodes_a: set<BLSPubkey>, h_nodes_a': set<BLSPubkey> :: 
-                                inv_exists_honest_node_that_contributed_to_decisions_of_consensus_instances(dv, a, a', m, consa, consa', h_nodes_a, h_nodes_a') ); 
-    }
-
-        // Wrong: 1st try in a new version
-//     lemma lem_no_slashable_submitted_attestations_with_different_slots_ii(
-//                 dv: DVState, 
-//                 a: Attestation, 
-//                 a': Attestation
-//     )
-//     requires inv_quorum_constraints(dv)    
-//     requires inv_exists_honest_node_that_contributed_to_creation_of_submitted_attestations_body(dv, a, a')
-//     requires inv_if_honest_node_sends_att_share_it_receives_att_data_before(dv)
-//     ensures && !is_slashable_attestation_data_eth_spec(a.data, a'.data)
-//             && !is_slashable_attestation_data_eth_spec(a'.data, a.data)
-//     {    
-//         var hn: BLSPubkey, att_shares: set<AttestationShare>, att_shares': set<AttestationShare> :|
-//                 && is_honest_node(dv, hn)
-//                 && pred_attestation_is_created_based_on_sent_attestation_shares(dv, a, att_shares)
-//                 && pred_is_owner_of_one_attestaion_share_in_set_of_shares(dv.honest_nodes_states[hn], att_shares)
-//                 && pred_attestation_is_created_based_on_sent_attestation_shares(dv, a', att_shares')
-//                 && pred_is_owner_of_one_attestaion_share_in_set_of_shares(dv.honest_nodes_states[hn], att_shares')
-//                 ;
-//         var dvc: DVCState := dv.honest_nodes_states[hn];
-//         var att_share: AttestationShare :| 
-//                 && att_share in att_shares 
-//                 && pred_verify_owner_of_attestation_share_with_bls_signature(dvc, att_share)
-//                 ;
-//         var att_share': AttestationShare :| 
-//                 && att_share' in att_shares' 
-//                 && pred_verify_owner_of_attestation_share_with_bls_signature(dvc, att_share')
-//                 ;
-
-//         assert inv_if_honest_node_sends_att_share_it_receives_att_data_before_body(dvc, att_share);
-//         assert inv_if_honest_node_sends_att_share_it_receives_att_data_before_body(dvc, att_share');
-
-//         var att_data: AttestationData := att_share.data;
-//         var slot: Slot := att_data.slot;
-//         var att_duty: AttestationDuty, vp: AttestationData -> bool :|
-//                 && att_duty in dvc.all_rcvd_duties
-//                 && slot in dvc.attestation_consensus_engine_state.att_slashing_db_hist.Keys
-//                 && vp in dvc.attestation_consensus_engine_state.att_slashing_db_hist[slot].Keys
-//                 // && consensus_is_valid_attestation_data(dvc.attestation_slashing_db, att_data, att_duty)
-//                 && vp(att_data)
-//                 ;
-
-//         assert consensus_is_valid_attestation_data(dvc.attestation_slashing_db, att_data, att_duty);
-
-//         var att_data': AttestationData := att_share'.data;
-//         var slot': Slot := att_data'.slot;
-//         var att_duty': AttestationDuty, vp': AttestationData -> bool :|
-//                 && att_duty' in dvc.all_rcvd_duties
-//                 && slot' in dvc.attestation_consensus_engine_state.att_slashing_db_hist.Keys
-//                 && vp' in dvc.attestation_consensus_engine_state.att_slashing_db_hist[slot'].Keys
-//                 // && consensus_is_valid_attestation_data(dvc.attestation_slashing_db, att_data', att_duty')
-//                 && vp'(att_data')
-//                 ;
-
-//         // assert  && !is_slashable_attestation_data_eth_spec(a.data, a'.data)
-//         //         && !is_slashable_attestation_data_eth_spec(a'.data, a.data)
-//         //         ;
-//     }
-
-        // Wrong: proof in the old version
-    lemma lem_no_slashable_submitted_attestations_with_different_slots_ii(
-                dv: DVState, 
-                a: Attestation, 
-                a': Attestation, 
-                m: BLSPubkey, 
-                consa: ConsensusInstance<AttestationData>, consa': ConsensusInstance<AttestationData>,
-                h_nodes_a: set<BLSPubkey>, h_nodes_a': set<BLSPubkey>)
-    requires |dv.all_nodes| > 0
-    requires inv_quorum_constraints(dv)    
-    requires inv_exists_honest_node_that_contributed_to_decisions_of_consensus_instances(dv, a, a', m, consa, consa', h_nodes_a, h_nodes_a')
-    requires && consa.decided_value.isPresent()
-             && consa'.decided_value.isPresent()
-             && a.data == consa.decided_value.safe_get()
-             && a'.data == consa'.decided_value.safe_get()
-    requires a.data.slot < a'.data.slot
-    requires inv_sent_validity_predicate_only_for_slots_stored_in_att_slashing_db_hist(dv)
-    requires inv_all_validity_predicates_are_stored_in_att_slashing_db_hist(dv)
-    requires inv_sent_validity_predicate_is_based_on_rcvd_att_duty_and_slashing_db(dv)
-    requires inv_sent_vp_is_based_on_existing_slashing_db_and_rcvd_att_duty(dv)
-    requires inv_slashing_db_att_in_db_for_low_slot_is_in_db_for_high_slot(dv)
-//     ensures && !is_slashable_attestation_data_eth_spec(a.data, a'.data)
-//             && !is_slashable_attestation_data_eth_spec(a'.data, a.data)
-    {    
-        assert  && is_a_valid_decided_value_according_to_set_of_nodes(consa, h_nodes_a)
-                && m in h_nodes_a
-                ;
-        assert  && is_a_valid_decided_value_according_to_set_of_nodes(consa', h_nodes_a')
-                && m in h_nodes_a'       
-                ;
-        
-        var m_state := dv.honest_nodes_states[m];
-        var slot_a := a.data.slot;
-        var slot_a' := a'.data.slot;
-
-        assert consa == dv.consensus_on_attestation_data[slot_a];
-        assert consa' == dv.consensus_on_attestation_data[slot_a'];
-
-        var dva := consa.decided_value.safe_get();
-        var dva' := consa'.decided_value.safe_get();
-        var sdba := construct_SlashingDBAttestation_from_att_data(dva);
-        var sdba' := construct_SlashingDBAttestation_from_att_data(dva');
-        
-        assert consa.honest_nodes_validity_functions[m] != {};
-        var vpa: AttestationData -> bool :| && vpa in consa.honest_nodes_validity_functions[m]
-                                            && vpa(dva);
-        
-        assert inv_all_validity_predicates_are_stored_in_att_slashing_db_hist_body(dv, m, m_state, slot_a, vpa);
-        assert vpa in m_state.attestation_consensus_engine_state.att_slashing_db_hist[slot_a];
-        var duty: AttestationDuty, dba :| inv_sent_vp_is_based_on_existing_slashing_db_and_rcvd_att_duty_body(dv, m, slot_a, dba, duty, vpa);
-        assert sdba in dba;
-
-        assert consa'.honest_nodes_validity_functions[m] != {};
-        var vpa': AttestationData -> bool :| && vpa' in consa'.honest_nodes_validity_functions[m]
-                                             && vpa'(dva');
-        assert inv_all_validity_predicates_are_stored_in_att_slashing_db_hist_body(dv, m, m_state, slot_a', vpa');
-        assert vpa' in m_state.attestation_consensus_engine_state.att_slashing_db_hist[slot_a'];
-        var duty': AttestationDuty, dba' :| inv_sent_vp_is_based_on_existing_slashing_db_and_rcvd_att_duty_body(dv, m, slot_a', dba', duty', vpa');
-        
-        assert inv_sent_vp_is_based_on_existing_slashing_db_and_rcvd_att_duty_body(dv, m, slot_a', dba', duty', vpa');
-        assert vpa' == (ad': AttestationData) => consensus_is_valid_attestation_data(dba', ad', duty');
-        assert !is_slashable_attestation_data(dba', dva');
-
-    
-        // Error
-        // lem_is_slashable_attestation_data(dba', dva', sdba, sdba');     
-
-        // assert !is_slashable_attestation_data_eth_spec(dva, dva');
-        // assert !is_slashable_attestation_data_eth_spec(dva', dva);                 
-    }
-
-
-        // 2nd try in a new version
-//     lemma lem_no_slashable_submitted_attestations_with_different_slots_ii(
-//                 dv: DVState, 
-//                 a: Attestation, 
-//                 a': Attestation, 
-//                 m: BLSPubkey, 
-//                 consa: ConsensusInstance<AttestationData>, consa': ConsensusInstance<AttestationData>,
-//                 h_nodes_a: set<BLSPubkey>, h_nodes_a': set<BLSPubkey>)
-//     requires |dv.all_nodes| > 0
-//     requires inv_quorum_constraints(dv)    
-//     requires inv_exists_honest_node_that_contributed_to_decisions_of_consensus_instances(dv, a, a', m, consa, consa', h_nodes_a, h_nodes_a')
-//     requires && consa.decided_value.isPresent()
-//              && consa'.decided_value.isPresent()
-//              && a.data == consa.decided_value.safe_get()
-//              && a'.data == consa'.decided_value.safe_get()
-//     requires a.data.slot < a'.data.slot
-//     requires inv_sent_validity_predicate_only_for_slots_stored_in_att_slashing_db_hist(dv)
-//     requires inv_all_validity_predicates_are_stored_in_att_slashing_db_hist(dv)
-//     requires inv_sent_validity_predicate_is_based_on_rcvd_att_duty_and_slashing_db(dv)
-//     requires inv_sent_vp_is_based_on_existing_slashing_db_and_rcvd_att_duty(dv)
-
-//     requires inv_attestation_is_created_with_shares_from_quorum(dv)
-//     requires inv_decided_value_of_consensus_instance_is_decided_by_quorum(dv)
-//     requires inv_db_of_vp_contains_all_att_data_of_sent_att_shares_for_lower_slots(dv)
-//     // requires pred_intersection_of_honest_nodes_in_two_quorum_contains_an_honest_node
-
-
-// //     ensures && !is_slashable_attestation_data_eth_spec(a.data, a'.data)
-// //             && !is_slashable_attestation_data_eth_spec(a'.data, a.data)
-//     {    
-//         assert  && is_a_valid_decided_value_according_to_set_of_nodes(consa, h_nodes_a)
-//                 && m in h_nodes_a
-//                 ;
-//         assert  && is_a_valid_decided_value_according_to_set_of_nodes(consa', h_nodes_a')
-//                 && m in h_nodes_a'       
-//                 ;
-        
-//         var m_state := dv.honest_nodes_states[m];
-//         var slot_a := a.data.slot;
-//         var slot_a' := a'.data.slot;
-
-//         assert consa == dv.consensus_on_attestation_data[slot_a];
-//         assert consa' == dv.consensus_on_attestation_data[slot_a'];
-
-//         var dva := consa.decided_value.safe_get();
-//         var dva' := consa'.decided_value.safe_get();
-//         var sdba := construct_SlashingDBAttestation_from_att_data(dva);
-//         var sdba' := construct_SlashingDBAttestation_from_att_data(dva');
-        
-//         assert consa.honest_nodes_validity_functions[m] != {};
-//         var vpa: AttestationData -> bool :| && vpa in consa.honest_nodes_validity_functions[m]
-//                                             && vpa(dva);
-        
-//         assert inv_all_validity_predicates_are_stored_in_att_slashing_db_hist_body(dv, m, m_state, slot_a, vpa);
-//         assert vpa in m_state.attestation_consensus_engine_state.att_slashing_db_hist[slot_a];
-//         var duty: AttestationDuty, dba :| inv_sent_vp_is_based_on_existing_slashing_db_and_rcvd_att_duty_body(dv, m, slot_a, dba, duty, vpa);
-//         assert sdba in dba;
-
-//         assert consa'.honest_nodes_validity_functions[m] != {};
-//         var vpa': AttestationData -> bool :| && vpa' in consa'.honest_nodes_validity_functions[m]
-//                                              && vpa'(dva');
-//         assert inv_all_validity_predicates_are_stored_in_att_slashing_db_hist_body(dv, m, m_state, slot_a', vpa');
-//         assert vpa' in m_state.attestation_consensus_engine_state.att_slashing_db_hist[slot_a'];
-//         var duty': AttestationDuty, dba' :| inv_sent_vp_is_based_on_existing_slashing_db_and_rcvd_att_duty_body(dv, m, slot_a', dba', duty', vpa');
-        
-//         assert inv_sent_vp_is_based_on_existing_slashing_db_and_rcvd_att_duty_body(dv, m, slot_a', dba', duty', vpa');
-//         assert vpa' == (ad': AttestationData) => consensus_is_valid_attestation_data(dba', ad', duty');
-//         assert !is_slashable_attestation_data(dba', dva');
-
-    
-//         // Error
-//         // lem_is_slashable_attestation_data(dba', dva', sdba, sdba');     
-
-//         // assert !is_slashable_attestation_data_eth_spec(dva, dva');
-//         // assert !is_slashable_attestation_data_eth_spec(dva', dva);                 
-//     }
-
-    // lemma lem_no_slashable_submitted_attestations_with_different_slots(dv: DVState, a: Attestation, a': Attestation)
-    // requires |dv.all_nodes| > 0
-    // requires inv_quorum_constraints(dv)
-    // requires inv_unchanged_paras_of_consensus_instances(dv)
-    // requires inv_exists_honest_dvc_that_sent_att_share_for_submitted_att(dv)
-    // requires inv_data_of_att_share_is_decided_value(dv)
-    // requires inv_decided_value_of_consensus_instance_is_decided_by_quorum(dv)    
-    // requires inv_sent_validity_predicate_is_based_on_rcvd_att_duty_and_slashing_db(dv)
-    // requires && a in dv.all_attestations_created
-    //          && is_valid_attestation(a, dv.dv_pubkey)
-    // requires && a' in dv.all_attestations_created
-    //          && is_valid_attestation(a', dv.dv_pubkey)
-    // requires a.data.slot < a'.data.slot 
-    // requires inv_decided_data_has_an_honest_witness(dv)
-    // requires inv_sent_validity_predicate_only_for_slots_stored_in_att_slashing_db_hist(dv)
-    // requires inv_all_validity_predicates_are_stored_in_att_slashing_db_hist(dv)
-    // requires inv_sent_vp_is_based_on_existing_slashing_db_and_rcvd_att_duty(dv)
-    // requires inv_unique_rcvd_att_duty_per_slot(dv)
-    // requires inv_active_consensus_instances_implied_the_delivery_of_att_duties(dv)
-    // requires inv_data_of_all_created_attestations_is_set_of_decided_values(dv)
-
-    // requires inv_exists_honest_node_that_contributed_to_creation_of_submitted_attestations_body(dv, a, a')
-    // requires inv_if_honest_node_sends_att_share_it_receives_att_data_before(dv)
-    // ensures && !is_slashable_attestation_data_eth_spec(a.data, a'.data)
-    //         && !is_slashable_attestation_data_eth_spec(a'.data, a.data)
-    // {
-    //     // lem_no_slashable_submitted_attestations_with_different_slots_i(dv, a, a');
-        
-    //     // var consa := dv.consensus_on_attestation_data[a.data.slot];
-    //     // var consa' := dv.consensus_on_attestation_data[a'.data.slot];                      
-    //     // var m: BLSPubkey, h_nodes_a: set<BLSPubkey>, h_nodes_a': set<BLSPubkey> :| 
-    //     //         inv_exists_honest_node_that_contributed_to_decisions_of_consensus_instances(dv, a, a', m, consa, consa', h_nodes_a, h_nodes_a');
-
-    //     // assert  inv_exists_honest_node_that_contributed_to_decisions_of_consensus_instances(dv, a, a', m, consa, consa', h_nodes_a, h_nodes_a');
-    //     // assert  && consa.decided_value.isPresent()
-    //     //         && consa'.decided_value.isPresent()
-    //     //         ;
-    //     // assert  && a.data == consa.decided_value.safe_get()
-    //     //         && a'.data == consa'.decided_value.safe_get()
-    //     //         ;
-
-    //     // lem_no_slashable_submitted_attestations_with_different_slots_ii(dv, a, a');
-    // }    
-
     lemma lem_no_slashable_submitted_attestations_with_different_slots(dv: DVState, a: Attestation, a': Attestation)
-    requires |dv.all_nodes| > 0
     requires inv_quorum_constraints(dv)
     requires inv_unchanged_paras_of_consensus_instances(dv)
     requires inv_exists_honest_dvc_that_sent_att_share_for_submitted_att(dv)
@@ -396,19 +70,18 @@ module Core_Proofs
     requires inv_sent_validity_predicate_only_for_slots_stored_in_att_slashing_db_hist(dv)
     requires inv_all_validity_predicates_are_stored_in_att_slashing_db_hist(dv)
     requires inv_sent_vp_is_based_on_existing_slashing_db_and_rcvd_att_duty(dv)
+    requires inv_data_of_all_created_attestations_is_set_of_decided_values(dv)
     requires inv_unique_rcvd_att_duty_per_slot(dv)
     requires inv_active_consensus_instances_implied_the_delivery_of_att_duties(dv)
-    requires inv_data_of_all_created_attestations_is_set_of_decided_values(dv)
-
     requires inv_attestation_is_created_with_shares_from_quorum(dv)
     requires inv_decided_value_of_consensus_instance_is_decided_by_quorum(dv)
     requires inv_db_of_vp_contains_all_att_data_of_sent_att_shares_for_lower_slots(dv)
     requires inv_unchanged_paras_of_consensus_instances(dv)
     requires inv_exists_db_in_att_slashing_db_hist_and_duty_for_every_validity_predicate(dv)
     requires inv_slots_for_sent_validity_predicate_are_stored_in_att_slashing_db_hist(dv)
-    // ensures && !is_slashable_attestation_data_eth_spec(a.data, a'.data)
-    //         && !is_slashable_attestation_data_eth_spec(a'.data, a.data)
-    {
+    ensures && !is_slashable_attestation_data_eth_spec(a.data, a'.data)
+            && !is_slashable_attestation_data_eth_spec(a'.data, a.data)
+    {        
         var data := a.data;
         var data' := a'.data;
         var slot: Slot := data.slot;
@@ -420,9 +93,18 @@ module Core_Proofs
         var sdba := construct_SlashingDBAttestation_from_att_data(dva);
         var sdba' := construct_SlashingDBAttestation_from_att_data(dva');
 
-        var att_shares: set<AttestationShare>, signers: set<BLSPubkey> :| inv_attestation_is_created_with_shares_from_quorum_body(dv, a, att_shares, signers);            
+        var att_shares: set<AttestationShare>, signers: set<BLSPubkey> :| 
+                && att_shares <= dv.att_network.allMessagesSent
+                && var constructed_sig := dv.construct_signed_attestation_signature(att_shares);
+                && constructed_sig.isPresent()
+                && constructed_sig.safe_get() == a.signature
+                && do_all_att_shares_have_the_same_data(att_shares, a.data)
+                && signers <= dv.all_nodes
+                && inv_attestation_is_created_with_shares_from_quorum_body_signers(att_shares, signers)
+                && |signers| >= quorum(|dv.all_nodes|)
+                ;
         assert  && signers <= dv.all_nodes
-                && inv_attestation_is_created_with_shares_from_quorum_body_signers(dv, att_shares, signers)
+                && inv_attestation_is_created_with_shares_from_quorum_body_signers(att_shares, signers)
                 && |signers| >= quorum(|dv.all_nodes|)           
             ;
 
@@ -463,7 +145,6 @@ module Core_Proofs
                 ;
         assert  is_honest_node(dv, m);
         assert  inv_attestation_is_created_with_shares_from_quorum_body_signers_helper(
-                    dv, 
                     att_shares,
                     m
                 );
@@ -516,23 +197,9 @@ module Core_Proofs
         assert  && !is_slashable_attestation_data_eth_spec(a.data, a'.data)
                 && !is_slashable_attestation_data_eth_spec(a'.data, a.data)
                 ;
-
-
-        // var m: BLSPubkey, h_nodes_a: set<BLSPubkey>, h_nodes_a': set<BLSPubkey> :| 
-        //         inv_exists_honest_node_that_contributed_to_decisions_of_consensus_instances(dv, a, a', m, consa, consa', h_nodes_a, h_nodes_a');
-
-        // assert  inv_exists_honest_node_that_contributed_to_decisions_of_consensus_instances(dv, a, a', m, consa, consa', h_nodes_a, h_nodes_a');
-        // assert  && consa.decided_value.isPresent()
-        //         && consa'.decided_value.isPresent()
-        //         ;
-        // assert  && a.data == consa.decided_value.safe_get()
-        //         && a'.data == consa'.decided_value.safe_get()
-        //         ;
-
     } 
 
     lemma lem_no_slashable_submitted_attestations_with_same_slots(dv: DVState, a: Attestation, a': Attestation)
-    requires |dv.all_nodes| > 0
     requires inv_quorum_constraints(dv)
     requires inv_unchanged_paras_of_consensus_instances(dv)
     requires inv_exists_honest_dvc_that_sent_att_share_for_submitted_att(dv)
@@ -552,14 +219,14 @@ module Core_Proofs
                 && att_share in dv.att_network.allMessagesSent
                 && att_share.data == a.data
                 && var attestation_signing_root := compute_attestation_signing_root(att_share.data, fv);
-                && verify_bls_siganture(attestation_signing_root, att_share.signature, hna);     
+                && verify_bls_signature(attestation_signing_root, att_share.signature, hna);     
 
         var hna', att_share', fv' :|
                 && hna' in dv.honest_nodes_states.Keys 
                 && att_share' in dv.att_network.allMessagesSent
                 && att_share'.data == a'.data
                 && var attestation_signing_root := compute_attestation_signing_root(att_share'.data, fv');
-                && verify_bls_siganture(attestation_signing_root, att_share'.signature, hna');   
+                && verify_bls_signature(attestation_signing_root, att_share'.signature, hna');   
 
         var cons := dv.consensus_on_attestation_data[a.data.slot];                 
 
@@ -574,7 +241,6 @@ module Core_Proofs
     }      
 
     lemma lem_no_slashable_submitted_attestations(dv: DVState, a: Attestation, a': Attestation)    
-    requires |dv.all_nodes| > 0
     requires inv_quorum_constraints(dv)
     requires inv_unchanged_paras_of_consensus_instances(dv)
     requires inv_exists_honest_dvc_that_sent_att_share_for_submitted_att(dv)
@@ -592,9 +258,12 @@ module Core_Proofs
     requires inv_unique_rcvd_att_duty_per_slot(dv)
     requires inv_active_consensus_instances_implied_the_delivery_of_att_duties(dv)
     requires inv_data_of_all_created_attestations_is_set_of_decided_values(dv)
-    
-    requires inv_exists_honest_node_that_contributed_to_creation_of_submitted_attestations_body(dv, a, a')
-    requires inv_if_honest_node_sends_att_share_it_receives_att_data_before(dv)        
+    requires inv_decided_value_of_consensus_instance_is_decided_by_quorum(dv)
+    requires inv_unchanged_paras_of_consensus_instances(dv)
+    requires inv_exists_db_in_att_slashing_db_hist_and_duty_for_every_validity_predicate(dv)
+    requires inv_slots_for_sent_validity_predicate_are_stored_in_att_slashing_db_hist(dv)
+    requires inv_attestation_is_created_with_shares_from_quorum(dv)
+    requires inv_db_of_vp_contains_all_att_data_of_sent_att_shares_for_lower_slots(dv)
     ensures && !is_slashable_attestation_data_eth_spec(a.data, a'.data)
             && !is_slashable_attestation_data_eth_spec(a'.data, a.data)   
     {
